books/projects/rp-rewriter/lib/mult3/spec-meta.lisp
@@ -1,0 +1,417 @@
+
+;; Mertcan Temel
+
+
+(in-package "RP")
+(include-book "svl-spec")
+
+(local
+ (include-book "projects/rp-rewriter/proofs/aux-function-lemmas" :dir :system))
+
+(local
+ (include-book "projects/rp-rewriter/proofs/eval-functions-lemmas" :dir :system))
+
+(local
+ (include-book "projects/rp-rewriter/proofs/rp-equal-lemmas" :dir :system))
+
+#|(local
+ (include-book "projects/rp-rewriter/proofs/rp-rw-lemmas" :dir :system))|#
+
+(local
+ (fetch-new-events
+  (include-book "arithmetic-5/top" :dir :system)
+  use-arith-5
+  :disabled t))
+
+(local
+ (rp::fetch-new-events
+  (include-book "centaur/bitops/ihs-extensions" :dir :system)
+  use-ihs-extensions
+  :disabled t))
+
+(local
+ (include-book "pp-flatten-meta-correct"))
+
+(local
+ (include-book "sum-merge-fncs-correct"))
+
+(local
+ (include-book "lemmas"))
+(local
+ (include-book "lemmas-2"))
+
+
+
+#|
+(BINARY-* (ACL2::RP 'INTEGERP
+                    (SVL::4VEC-CONCAT$ '23
+                                       (SVL::BITS (ACL2::RP 'INTEGERP SRC1)
+                                                  '0
+                                                  '23)
+                                       '1))
+          (ACL2::RP 'INTEGERP
+                    (SVL::4VEC-CONCAT$ '23
+                                       (SVL::BITS (ACL2::RP 'INTEGERP SRC2)
+                                                  '0
+                                                  '23)
+'1)))
+
+|#
+
+(define check-context-for-integerp (term context)
+  (if (atom context)
+      nil
+    (or (b* ((cur (ex-from-rp (car context))))
+          (case-match cur
+            (('integerp x)
+             (rp-equal-cnt term x 1))))
+        (check-context-for-integerp term (cdr context)))))
+
+(define logsize ((x integerp))
+  :prepwork ((local
+              (use-arith-5 t))
+             (local
+              (in-theory (e/d* ()
+                               (rw-dir1
+                                +-IS-SUM
+                                FLOOR2-IF-F2)))))
+  (if (or (equal x 0)
+          (equal x -1)
+          (not (integerp x)))
+      0
+    (1+ (logsize (acl2::logcdr x)))))
+
+(define calculate-vec-size ((x rp-termp)
+                            (context rp-term-listp))
+  :returns (mv (size integerp)
+               (integerp booleanp))
+  :verify-guards :after-returns
+  :measure (cons-count x)
+  :hints (("Goal"
+           :in-theory (e/d (measure-lemmas
+                            ACL2::DEFSORT-O<-OF-NATURALS)
+                           (RW->-TO-GT
+                            (:REWRITE LT-TO-GT)
+                            (:REWRITE RW-<-TO-LTE)))))
+  (b* ((x (ex-from-rp x)))
+    (case-match x
+      (('svl::bits vec ('quote start) ('quote size))
+       (b* (((unless (and (natp start)
+                          (natp size)))
+             (mv -1 nil))
+            ((mv & integerp)
+             (calculate-vec-size vec context)))
+         (mv size integerp)))
+      (('svl::4vec-concat$ ('quote size) vec1 vec2)
+       (b* (((mv & integerp1)
+             (calculate-vec-size vec1 context))
+            ((mv size2 integerp2)
+             (calculate-vec-size vec2 context))
+            ((unless (and integerp1
+                          integerp2
+                          (not (equal size2 -1))
+                          (natp size)))
+             (mv -1 nil)))
+         (mv (+ size size2) t)))
+      (('quote x)
+       (if (natp x)
+           (mv (logsize x) t)
+         (mv -1 nil)))
+      (&
+       (if (atom x)
+           (mv -1 (check-context-for-integerp x context))
+         (mv -1 nil))))))
+
+#|(calculate-vec-size '(ACL2::RP 'INTEGERP
+                               (SVL::4VEC-CONCAT$ '23
+                                                  (SVL::BITS (ACL2::RP 'INTEGERP SRC1)
+                                                             '0
+                                                             '23)
+                                                  '1))
+                    '((integerp src1)))|#
+
+(define *-to-mult-spec-meta ((term rp-termp)
+                             (context rp-term-listp))
+  (case-match term
+    (('binary-* x y)
+     (b* (((mv size-x integerp-x)
+           (calculate-vec-size x context))
+          ((mv size-y integerp-y)
+           (calculate-vec-size y context))
+          ((unless (and integerp-x
+                        (not (equal size-x -1))
+                        (not (equal size-y -1))
+                        integerp-y))
+           (mv term nil)))
+       (mv `(svl-mult-final-spec ,x ,y ',(+ size-x size-y))
+           `(nil t t t))))
+    (& (mv term nil))))
+
+#|(*-to-mult-spec-meta  '(BINARY-* (ACL2::RP 'INTEGERP
+                                           (SVL::4VEC-CONCAT$ '23
+                                                              (SVL::BITS (ACL2::RP 'INTEGERP SRC1)
+                                                                         '0
+                                                                         '23)
+                                                              '1))
+                                 (ACL2::RP 'INTEGERP
+                                           (SVL::4VEC-CONCAT$ '23
+                                                              (SVL::BITS (ACL2::RP 'INTEGERP SRC2)
+                                                                         '0
+                                                                         '23)
+                                                              '1)))
+                      '((integerp src1)
+                        (integerp src2)))|#
+
+(encapsulate
+  nil
+  (local
+   (in-theory
+    (e/d* () (+-IS-SUM
+              REWRITING-POSITIVE-LTE-GTE-GT-LT
+              rw-dir1
+              C-SPEC-IS-F2
+              S-SPEC-IS-M2
+              S-C-SPEC-IS-LIST-M2-F2
+              SVL::4VEC-ZERO-EXT-IS-4VEC-CONCAT
+              SVL-SUM-PPS-BYCOL-BYBIT-OPENER))))
+  (with-output
+    :off :all
+    :gag-mode nil
+    (rp::def-formula-checks *-to-mult-spec-meta-fchecks
+      (svl::bits svl::4vec-concat$ *
+                 SVL-MULT-FINAL-SPEC))))
+
+(local
+ (progn
+   (rp::create-regular-eval-lemma svl::4VEC-CONCAT$ 3
+                                  *-to-mult-spec-meta-fchecks)
+   (rp::create-regular-eval-lemma SVL-MULT-FINAL-SPEC 3  *-to-mult-spec-meta-fchecks)
+   (rp::create-regular-eval-lemma svl::Bits 3  *-to-mult-spec-meta-fchecks)
+   (rp::create-regular-eval-lemma binary-* 2  *-to-mult-spec-meta-fchecks)
+   (rp::create-regular-eval-lemma integerp 1  *-to-mult-spec-meta-fchecks)))
+
+(local
+ (defthm CHECK-CONTEXT-FOR-INTEGERP-correct
+   (implies (and (eval-and-all context a)
+                 (rp-evl-meta-extract-global-facts)
+                 (*-to-mult-spec-meta-fchecks state)
+                 (check-context-for-integerp term context))
+            (integerp (rp-evlt term a)))
+   :hints (("Subgoal *1/2"
+            :use ((:instance rp-evlt-of-rp-equal
+                             (term1 term)
+                             (term2 (CADR (EX-FROM-RP (CAR CONTEXT)))))))
+           ("Goal"
+            :in-theory (e/d* (check-context-for-integerp
+                              RP-EVLT-OF-EX-FROM-RP-REVERSE
+                              regular-eval-lemmas
+                              regular-eval-lemmas-with-ex-from-rp)
+                             (rp-evlt-of-rp-equal
+                              rp-evlt-of-ex-from-rp ))))))
+
+(local
+ (defthm rp-evlt-when-quoted
+   (implies (and (quotep term)
+                 (consp (cdr term)))
+            (equal (rp-evlt term a)
+                   (cadr term)))))
+
+
+(defthm unsigned-byte-p-of-logsize
+  (implies (natp x)
+           (unsigned-byte-p (logsize x)
+                            x))
+  :hints (("Goal"
+           :in-theory (e/d* (unsigned-byte-p-redef-to-recursive
+                             ;;bitops::ihsext-inductions
+                             ;;bitops::ihsext-recursive-redefs
+                             logsize
+                             )
+                            (rw-dir1
+                             LOGCOUNT
+                             (:induction UNSIGNED-BYTE-P-RECURSIVE)
+                             acl2::logcdr
+                             acl2::logcar
+                             +-IS-SUM)))))
+
+
+(local
+ (defthm unsigned-byte-p-of-logapp
+   (implies (and (natp size)
+                 (natp size2)
+                 ;;(<= size2 size)
+                 (integerp y)
+                 (integerp x))
+            (equal (unsigned-byte-p (+ size2 size) (logapp size2 x y))
+                   (unsigned-byte-p size y)))
+   :hints (("Goal"
+            :do-not-induct t
+            :induct (unsigned-byte-p-recursive size2 x)
+            :expand ((LOGAPP SIZE2 0 Y)
+                     (UNSIGNED-BYTE-P-RECURSIVE SIZE
+                                 (ACL2::LOGCONS 0 (LOGAPP (+ -1 SIZE2) 0 Y))))
+            :in-theory (e/d* (SVL::4VEC-CONCAT$
+                              BITOPS::LOGCDR-OF-LOGCONS
+                              unsigned-byte-p-redef-to-recursive
+                              acl2::logapp**
+                              SV::4VEC-CONCAT
+                              ;;bitops::ihsext-inductions
+                              bitops::ihsext-recursive-redefs
+                              natp
+                              SV::4VEC->UPPER
+                              SV::4VEC->lower
+                              SV::4VEC)
+                             (+-IS-SUM
+                              ACL2::LOGCONS$INLINE
+                              MOD2-IS-M2
+                              acl2::logcdr
+                              FLOOR
+                              FLOOR2-IF-F2
+                              unsigned-byte-p
+                              LOGAPP
+                              ACL2::LOGHEAD$INLINE
+                              rw-dir1))))))
+
+(local
+ (defthm unsigned-byte-p-of-4VEC-CONCAT$
+   (implies (and (natp size)
+                 (natp size2)
+                 (integerp x)
+                 (integerp y)
+                 (<= size2 size))
+            (equal (unsigned-byte-p size (SVL::4VEC-CONCAT$ size2 x y))
+                   (unsigned-byte-p (- size size2) y)))
+   :hints (("Goal"
+            :use ((:instance unsigned-byte-p-of-logapp
+                             (y y)
+                             (size (- size size2))
+                             (size2 size2)))
+            :do-not-induct t
+            :in-theory (e/d* (SVL::4VEC-CONCAT$
+                              unsigned-byte-p-redef-to-recursive
+                              
+                              SV::4VEC-CONCAT
+                              bitops::ihsext-inductions
+                              bitops::ihsext-recursive-redefs
+                              natp
+                              SV::4VEC->UPPER
+                              SV::4VEC->lower
+                              SV::4VEC)
+                             (+-IS-SUM
+                              unsigned-byte-p-of-logapp
+                              MOD2-IS-M2
+                              FLOOR
+                              FLOOR2-IF-F2
+                              unsigned-byte-p
+                              LOGAPP
+                              ACL2::LOGHEAD$INLINE
+                              rw-dir1))))))
+
+(local
+ (defthm dumy-sum-cancel-lemma
+   (implies (acl2-numberp other)
+            (and (equal (+ x (- x) other)
+                        other)))))
+(local
+ (defthm integerp-implies-acl2-numberp
+   (implies (integerp x)
+            (acl2-numberp x))))
+
+(local
+ (defthm natp-of-sums
+   (implies (and (NATP X)
+                 (natp y))
+            (natp (+ x y)))))
+
+(defret calculate-vec-size-correct
+  (implies (and (rp-evl-meta-extract-global-facts)
+                (eval-and-all context a)
+                (*-to-mult-spec-meta-fchecks state)
+                integerp)
+           (and (integerp (rp-evlt x a))
+                (integerp size)
+                (implies (not (equal size -1))
+                         (and (unsigned-byte-p size
+                                               (rp-evlt x a))
+                              (natp size)))))
+  :fn calculate-vec-size
+  :hints (("Subgoal *1/7"
+           :use ((:instance CHECK-CONTEXT-FOR-INTEGERP-correct
+                            (term (EX-FROM-RP X)))))
+          ("Goal"
+           :do-not-induct t
+           :induct (calculate-vec-size x context)
+           :in-theory (e/d* (calculate-vec-size
+                             natp
+                             RP-EVLT-OF-EX-FROM-RP-REVERSE
+                             regular-eval-lemmas
+                             regular-eval-lemmas-with-ex-from-rp)
+                            (UNSIGNED-BYTE-P
+                             RP-TERMP-IMPLIES-SUBTERMS
+                             RP-TERM-LISTP
+                             rw-dir1
+                             natp
+                             +-IS-SUM
+                             rp-trans
+                             INCLUDE-FNC
+                             rp-evlt-of-ex-from-rp
+                             CHECK-CONTEXT-FOR-INTEGERP-correct
+                             logcount)))))
+
+
+(defret *-to-mult-spec-meta-correct
+  (implies (and (rp-evl-meta-extract-global-facts)
+                (eval-and-all context a)
+                (*-to-mult-spec-meta-fchecks state))
+           (equal (rp-evlt (mv-nth 0 (*-to-mult-spec-meta term context)) a)
+                  (rp-evlt term a)))
+  :hints (("Goal"
+           :do-not-induct t
+           :use ((:instance *-of-known-sized-vecs
+                            (x (rp-evlt (cadr term) a))
+                            (y (rp-evlt (caddr term) a))
+                            (size1 (mv-nth 0
+                                           (calculate-vec-size (cadr term)
+                                                               context)))
+                            (size2 (mv-nth 0
+                                           (calculate-vec-size (caddr term)
+                                                               context)))))
+           :in-theory (e/d* (*-to-mult-spec-meta
+                             regular-eval-lemmas-with-ex-from-rp
+                             regular-eval-lemmas)
+                            (+-IS-SUM
+                             *-of-known-sized-vecs
+                             SVL-MULT-FINAL-SPEC
+                             RP-TRANS-LST
+                             rp-trans
+                             rw-dir1
+                             natp
+                             UNSIGNED-BYTE-P
+                             RP-TRANS-OPENER
+                             INCLUDE-FNC)))))
+
+(defret *-to-mult-spec-meta-valid-sc
+  (implies (valid-sc term a)
+           (valid-sc (mv-nth 0 (*-to-mult-spec-meta term context)) a))
+  :hints (("Goal"
+           :do-not-induct t
+           
+           :in-theory (e/d* (*-to-mult-spec-meta
+                             valid-sc is-rp is-if)
+                            ()))))
+
+(defret *-to-mult-spec-meta-rp-termp
+  (implies (rp-termp term)
+           (rp-termp (mv-nth 0 (*-to-mult-spec-meta term context))))
+  :hints (("Goal"
+           :do-not-induct t
+           
+           :in-theory (e/d* (*-to-mult-spec-meta
+                             valid-sc is-rp is-if)
+                            ()))))
+(rp::add-meta-rule
+ :meta-fnc *-to-mult-spec-meta
+ :trig-fnc binary-*
+ :valid-syntaxp t
+ :formula-checks *-to-mult-spec-meta-fchecks
+ :returns (mv term dont-rw))
